Azurite/AzNat/Conversion.lean
@@ -1,0 +1,45 @@
+import Azurite.AzNat.ToString
+
+def UInt64.toAzNat (u : UInt64) : Azurite.AzNat :=
+  if h : u = 0 then
+    ⟨#[], by simp⟩
+  else
+    ⟨#[u], by
+      intro hc
+      have h1 : #[u].back? = some u := rfl
+      rw [h1] at hc
+      simp at hc
+      contradiction⟩
+
+def UInt32.toAzNat (u : UInt32) : Azurite.AzNat := u.toUInt64.toAzNat
+def UInt16.toAzNat (u : UInt16) : Azurite.AzNat := u.toUInt64.toAzNat
+def UInt8.toAzNat (u : UInt8) : Azurite.AzNat := u.toUInt64.toAzNat
+def USize.toAzNat (u : USize) : Azurite.AzNat := u.toUInt64.toAzNat
+
+def Int64.toAzNatClampNeg (i : Int64) : Azurite.AzNat :=
+  if i < 0 then
+    ⟨#[], by simp⟩
+  else
+    i.toUInt64.toAzNat
+
+def Int32.toAzNatClampNeg (i : Int32) : Azurite.AzNat := i.toInt64.toAzNatClampNeg
+def Int16.toAzNatClampNeg (i : Int16) : Azurite.AzNat := i.toInt64.toAzNatClampNeg
+def Int8.toAzNatClampNeg (i : Int8) : Azurite.AzNat := i.toInt64.toAzNatClampNeg
+def ISize.toAzNatClampNeg (i : ISize) : Azurite.AzNat := i.toInt64.toAzNatClampNeg
+
+#guard toString (0 : UInt64).toAzNat == "0"
+#guard toString (5 : UInt64).toAzNat == "5"
+#guard toString (18446744073709551615 : UInt64).toAzNat == "18446744073709551615"
+
+#guard toString ((0 : Int64).toAzNatClampNeg) == "0"
+#guard toString ((-5 : Int64).toAzNatClampNeg) == "0"
+#guard toString ((-9223372036854775808 : Int64).toAzNatClampNeg) == "0"
+#guard toString ((5 : Int64).toAzNatClampNeg) == "5"
+#guard toString ((9223372036854775807 : Int64).toAzNatClampNeg) == "9223372036854775807"
+
+#guard toString ((0 : Int32).toAzNatClampNeg) == "0"
+#guard toString ((-5 : Int32).toAzNatClampNeg) == "0"
+#guard toString ((5 : Int32).toAzNatClampNeg) == "5"
+
+#guard toString ((-5 : ISize).toAzNatClampNeg) == "0"
+#guard toString ((5 : ISize).toAzNatClampNeg) == "5"
